Save.

src/CDCLtransition.v
@@ -13,19 +13,51 @@ Open Scope list_scope.
 (* Assignment Stack records the decision point and partial assignment *)
 (* The first PAssignment V is the guessed literal, the second is deduced literals *)
 (* Definition AssignmentStack (V: Set) := list ( PAssignment V * PAssignment V). *)
-(* We make it inductive type so that we have *)
-Inductive AssignmentStack {V:Set} : PAssignment V -> PAssignment V -> Set :=
+(* 
+Maintain the invariance that 
+  AS f (g,d)
+(f conj g) imply d
+*)
+(* We choose to use CNF to represent formula here
+    but in the resolution proof we uses Formula V to represent formula
+*)
+Inductive AssignmentStack {V:Set} (f : CNF V) : 
+  list (PAssignment V * PAssignment V) -> Set :=
   | empty_as : AssignmentStack ∅ ∅
   | guess_as : forall 
   | deduce_as :
+  | change_goal : 
+
+(* change_goal is used to implement learn and forget *)
 (* The invariant include the later one must 
   have consistent assignment as the
   former ones
 *)
 
+Notation "AS" := AssignmentStack.
+
 Definition LiteralsForm {V} (pa : PAssignment V) : Formula V. 
 Admitted.
 
+
+Proposition AssignmentStackHasRProof:
+  forall f g d,
+    AS f ((g,d):_) ->
+    RProof (conj f (LiteralsForm g)) (LiteralsForm d).
+Admitted.
+
+Proposition AssignmentStackCanWeaken:
+  forall f g d,
+  AS f s ->
+  RProof h f ->
+  AS h s.
+Admitted.
+
+Proposition AssignmentStackMonotoncity:
+  forall f g d,
+  AS f (t:s) ->
+  AS f s.
+Admitted.
 
 Definition RProofInv {V} 
     (orginal : Formula V) 
@@ -38,7 +70,7 @@ Fixpoint RProofInvAStack {V}
   match astack with
   | 
 
-Definition CDCLState {V : Set} :=  (AssignmentStack V) * (CNF V). 
+(* Definition CDCLState {V : Set} :=  (AssignmentStack V) * (CNF V).  *)
 
 (* Note that 
   CDCL are really doing proof search for undecdiability proof
@@ -46,9 +78,18 @@ Definition CDCLState {V : Set} :=  (AssignmentStack V) * (CNF V).
     Assignment
 *)
 
-Inductive FinalState {V : Set} : CDCLState (V := V) -> Prop :=
+(* Inductive FinalState {V : Set} : CDCLState (V := V) -> Prop :=
   | failst : forall a c, (CNFByPAssignment c a = Some false) -> FinalState (a::nil, c)
-  | succeedst : forall a b c, (CNFByPAssignment c a = Some true) -> FinalState (a::b, c).
+  | succeedst : forall a b c, (CNFByPAssignment c a = Some true) -> FinalState (a::b, c). *)
+
+Definition SucceedState := .
+
+
+Definition FailedState {V : Set} (st : AS f s)
+
+
+Definition FinalState {V : Set} (st : AS f s) := SucceedState st \/ FailedState st.
+
 
 
 (* We will have a non-determinism state transition machine
@@ -78,3 +119,40 @@ Proposition step_with_proof:
   forall x y,
     step (astack, fx) (bstack, fy) ->
 
+
+
+(* This is not so important but
+    we have a partial ordering on Assignment Stack
+    and if we have finite number of variables
+    i.e. V is of finite size, 
+    then we have, for every chain, a "largest" stack
+
+    This is not important because it is just a theorem/verification
+     we need to prove 
+
+    It will disappear after extraction.
+
+    The important is the four theorem that act as small-step transition
+    Basically unit prop, decide, checkFail, and backjump.
+
+    We might need to add more
+    *)
+Proposition Terminating:
+  forall x y,
+    steps x y ->
+    exists z,
+    steps y z /\ FinalState z.
+Admitted.
+
+
+(* The following are the extracted functions *)
+
+(* One step unit-prop *)
+
+(* UnitProp until cannot *)
+
+(* Guess One Literal *)
+
+(* Check Failure *)
+
+(* Back Jump *)
